New structure

src/linear/layer2/ArrayList.dfy
@@ -1,105 +1,5 @@
 include "../../Utils.dfy"
-include "../adt/List.dfy"
-
-
-trait ArrayListIterator extends ListIterator {
-  predicate Valid()
-    reads this, Parent(), Parent().Repr()
-
-  function Parent(): List
-    reads this
-    ensures Parent() is ArrayList
-
-  function Index() : nat
-    reads this, Parent(), Parent().Repr()
-    requires Valid()
-    requires Parent().Valid()
-    ensures Index() <= |Parent().Model()|
-
-  function method HasNext(): bool
-    reads this, Parent(), Parent().Repr()
-    requires Valid()
-    requires Parent().Valid()
-    ensures HasNext() <==> Index() < |Parent().Model()|
-
-  function method Peek(): int
-    reads this, Parent(), Parent().Repr()
-    requires Valid()
-    requires Parent().Valid()
-    requires HasNext()
-    ensures Peek() == Parent().Model()[Index()]
-
-  method Next() returns (x: int)
-    modifies this
-    requires Valid()
-    requires Parent().Valid()
-    requires HasNext()
-    requires allocated(Parent())
-    requires forall it | it in Parent().Repr() :: allocated(it)
-    ensures Parent().Valid()
-    ensures Valid()
-    ensures old(Parent()) == Parent()
-    ensures old(Parent().Model()) == Parent().Model()       // ?
-
-    ensures forall x {:trigger x in Parent().Repr(), x in old(Parent().Repr())} | x in Parent().Repr() - old(Parent().Repr()) :: fresh(x)
-    ensures fresh(Parent().Repr() - old(Parent().Repr()))
-    ensures forall x | x in Parent().Repr() :: allocated(x)
-
-    ensures Parent().Iterators() == old(Parent().Iterators())   // ?
-    ensures x == Parent().Model()[old(Index())]
-    ensures Index() == 1 + old(Index())
-    ensures forall it | it in Parent().Iterators() && old(it.Valid()) ::
-       it.Valid() && (it != this ==> it.Index() == old(it.Index()))
-
-  method Copy() returns (it: ListIterator)
-    modifies Parent(), Parent().Repr()
-    requires Valid()
-    requires Parent().Valid()
-    requires allocated(Parent())
-    requires forall it | it in Parent().Iterators() :: allocated(it)
-    ensures fresh(it)
-    ensures Valid()
-    ensures it.Valid()
-    ensures Parent().Valid()
-
-    ensures forall x {:trigger x in Parent().Repr(), x in old(Parent().Repr())} | x in Parent().Repr() - old(Parent().Repr()) :: fresh(x)
-    ensures fresh(Parent().Repr()-old(Parent().Repr()))
-    ensures forall x | x in Parent().Repr() :: allocated(x)
-
-    ensures it in Parent().Iterators()
-    ensures Parent().Iterators() == {it} + old(Parent().Iterators())
-    ensures Parent() == old(Parent())
-    ensures Parent() == it.Parent()
-    ensures Index() == it.Index()
-    ensures it.Valid()
-    ensures forall it | it in old(Parent().Iterators()) && old(it.Valid()) ::
-    it.Valid() && it.Index() == old(it.Index())
-    ensures Parent().Model() == old(Parent().Model())
-
-  method Set(x: int)
-    modifies Parent(), Parent().Repr()
-    requires Valid()
-    requires Parent().Valid()
-    requires allocated(Parent())
-    requires forall it | it in Parent().Repr() :: allocated(it)
-    requires HasNext()
-    ensures Valid()
-    ensures Parent().Valid()
-    ensures Parent() == old(Parent())
-
-    ensures forall x {:trigger x in Parent().Repr(), x in old(Parent().Repr())} | x in Parent().Repr() - old(Parent().Repr()) :: fresh(x)
-    ensures fresh(Parent().Repr()-old(Parent().Repr()))
-    ensures forall x | x in Parent().Repr() :: allocated(x)
-
-    ensures Parent().Iterators() == old(Parent().Iterators())
-    ensures forall it | it in old(Parent().Iterators()) && old(it.Valid()) ::
-      it.Valid() && it.Index() == old(it.Index())
-    ensures |Parent().Model()| == old(|Parent().Model()|)
-    ensures Index() == old(Index())
-    ensures Parent().Model()[Index()] == x
-    ensures forall i | 0 <= i < |Parent().Model()| && i != Index() ::
-      Parent().Model()[i] == old(Parent().Model()[i])
-}
+include "../layer1/List.dfy"
 
 
 trait ArrayList extends List {
@@ -195,26 +95,24 @@ trait ArrayList extends List {
     ensures Valid()
     ensures Model() == old(Model())
 
-    ensures it is ArrayListIterator
-    ensures fresh(it)
-    ensures it.Valid()
-    ensures it.Parent() == this
-    ensures it.Index() == 0
-
     ensures forall x {:trigger x in Repr(), x in old(Repr())} | x in Repr() - old(Repr()) :: fresh(x)
     ensures fresh(Repr() - old(Repr()))
     ensures forall x | x in Repr() :: allocated(x)
 
+    ensures fresh(it)
+    ensures it.Valid()
+    ensures it.Parent() == this
+    ensures it.Index() == 0
     ensures Iterators() == {it} + old(Iterators())
     ensures forall it | it in old(Iterators()) :: old(it.Valid())
       ==> it.Valid() && old(it.Parent()) == it.Parent() && old(it.Index()) == it.Index();
 
-  method Insert(mid: ListIterator, x: int)
+  // Insertion of x before mid, newt points to x
+  method Insert(mid: ListIterator, x: int) returns (newt:ListIterator)
     modifies this, Repr()
     requires Valid()
     requires mid.Valid()
     requires mid.Parent() == this
-    requires mid.HasNext()
     requires mid in Iterators()
     requires forall x | x in Repr() :: allocated(x)
 
@@ -225,10 +123,14 @@ trait ArrayList extends List {
     ensures fresh(Repr() - old(Repr()))
     ensures forall x | x in Repr() :: allocated(x)
 
-    ensures Iterators() == old(Iterators())
+    ensures fresh(newt)
+    ensures Iterators() == {newt}+old(Iterators())
+    ensures newt.Valid() && newt.Parent()==this && newt.Index()==old(mid.Index())
+ 
     ensures forall it | it in old(Iterators()) :: old(it.Valid())
       ==> it.Valid() && old(it.Parent()) == it.Parent() && old(it.Index()) == it.Index();
 
+  // Deletion of mid, next points to the next element (or past-the-end)
   method Erase(mid: ListIterator) returns (next: ListIterator)
     modifies this, Repr()
     requires Valid()
@@ -248,8 +150,9 @@ trait ArrayList extends List {
     ensures fresh(next)
     ensures Iterators() == {next} + old(Iterators())
     ensures forall it | it in old(Iterators()) :: old(it.Valid()) && old(it.HasNext())
-      ==> it.Valid() && old(it.Parent()) == it.Parent() && old(it.Index()) == it.Index();    
-    ensures next.Valid() && next.Parent() == this && next.Index() == mid.Index();
+      ==> it.Valid() && old(it.Parent()) == it.Parent() && old(it.Index()) == it.Index()
+    ensures next.Valid() && next.Parent() == this && next.Index() == mid.Index()
+
 }
 
 
