src/linear/layer2/LinkedList.dfy
@@ -1,5 +1,5 @@
 include "../../../src/Utils.dfy"
-include "../adt/List.dfy"
+include "../layer1/List.dfy"
 
 trait LinkedList extends List {
 
