src/linear/layer3/VectorImpl.dfy
@@ -1,7 +1,7 @@
-include "../../Utils.dfy"
-include "ArrayList.dfy"
+include "../../../src/Utils.dfy"
+include "../../../src/linear/layer2/Vector.dfy"
 
-class ArrayListIteratorImpl extends ListIterator {
+class ArrayListIteratorImpl extends ArrayListIterator {
   var parent: ArrayListImpl
   var index: nat
 
@@ -91,24 +91,26 @@ class ArrayListIteratorImpl extends ListIterator {
     requires forall it | it in Parent().Iterators() :: allocated(it)
     ensures fresh(it)
     ensures Valid()
-    ensures Parent() == old(Parent())
+    ensures it.Valid()
     ensures Parent().Valid()
-    ensures Parent().Model() == old(Parent().Model())
 
     ensures forall x {:trigger x in Parent().Repr(), x in old(Parent().Repr())} | x in Parent().Repr() - old(Parent().Repr()) :: fresh(x)
     ensures fresh(Parent().Repr()-old(Parent().Repr()))
     ensures forall x | x in Parent().Repr() :: allocated(x)
-    
-    ensures it.Valid()
+
+    ensures it in Parent().Iterators()
     ensures Parent().Iterators() == {it} + old(Parent().Iterators())
+    ensures Parent() == old(Parent())
     ensures Parent() == it.Parent()
     ensures Index() == it.Index()
+    ensures it.Valid()
     ensures forall it | it in old(Parent().Iterators()) && old(it.Valid()) ::
-      it.Valid() && it.Index() == old(it.Index())
+    it.Valid() && it.Index() == old(it.Index())
+    ensures Parent().Model() == old(Parent().Model())
     {
-      var itImpl := new ArrayListIteratorImpl(parent);      
+      var itImpl := new ArrayListIteratorImpl(parent);
       itImpl.index := index;
-      it := itImpl; 
+      it := itImpl;
       parent.iterators := parent.iterators + { itImpl };
     }
 
@@ -122,24 +124,23 @@ class ArrayListIteratorImpl extends ListIterator {
     ensures Valid()
     ensures Parent().Valid()
     ensures Parent() == old(Parent())
-    ensures |Parent().Model()| == old(|Parent().Model()|)
-    ensures Parent().Model()[old(Index())] == x
-    ensures forall i | 0 <= i < |Parent().Model()| && i != old(Index()) ::
-      Parent().Model()[i] == old(Parent().Model()[i])
 
     ensures forall x {:trigger x in Parent().Repr(), x in old(Parent().Repr())} | x in Parent().Repr() - old(Parent().Repr()) :: fresh(x)
     ensures fresh(Parent().Repr()-old(Parent().Repr()))
     ensures forall x | x in Parent().Repr() :: allocated(x)
 
-    //ensures Index() == old(Index())
     ensures Parent().Iterators() == old(Parent().Iterators())
     ensures forall it | it in old(Parent().Iterators()) && old(it.Valid()) ::
       it.Valid() && it.Index() == old(it.Index())
- {
+    ensures |Parent().Model()| == old(|Parent().Model()|)
+    ensures Index() == old(Index())
+    ensures Parent().Model()[Index()] == x
+    ensures forall i | 0 <= i < |Parent().Model()| && i != Index() ::
+      Parent().Model()[i] == old(Parent().Model()[i])
+  {
     parent.elements[index] := x;
   }
 }
-
 
 class ArrayListImpl extends ArrayList {
   var elements: array<int>;
@@ -195,7 +196,6 @@ class ArrayListImpl extends ArrayList {
     iterators
   }
 
-
   constructor()
     ensures Valid()
     ensures Model() == []
@@ -214,7 +214,6 @@ class ArrayListImpl extends ArrayList {
     size == 0
   }
 
-
   function method Size(): nat
     reads this, Repr()
     requires Valid()
@@ -223,12 +222,11 @@ class ArrayListImpl extends ArrayList {
     size
   }
 
-
   function method Front(): int
     reads this, Repr()
     requires Valid()
     requires Model() != []
-    
+
     ensures Valid()
     ensures Front() == Model()[0]
   {
@@ -239,7 +237,7 @@ class ArrayListImpl extends ArrayList {
     modifies this, Repr()
     requires Valid()
     requires forall x | x in Repr() :: allocated(x)
-    
+
     ensures Valid()
     ensures Model() == [x] + old(Model())
 
@@ -250,7 +248,7 @@ class ArrayListImpl extends ArrayList {
     ensures Iterators() == old(Iterators())
     ensures forall it | it in old(iterators) :: old(it.Valid())
       ==> it.Valid() && old(it.Parent()) == it.Parent() && old(it.Index()) == it.Index();
-  {      
+  {
     if (size == elements.Length) {
       Grow(elements.Length * 2);
     }
@@ -282,12 +280,11 @@ class ArrayListImpl extends ArrayList {
     size := size - 1;
   }
 
-
   function method Back(): int
     reads this, Repr()
     requires Valid()
     requires Model() != []
-    
+
     ensures Valid()
     ensures Back() == Model()[|Model()|-1]
   {
@@ -299,7 +296,7 @@ class ArrayListImpl extends ArrayList {
     requires Valid()
     requires Model() != []
     requires forall x | x in Repr() :: allocated(x)
-    
+
     ensures Valid()
     ensures Model() + [x] == old(Model())
 
@@ -316,12 +313,11 @@ class ArrayListImpl extends ArrayList {
     size := size - 1;
   }
 
-
   method PushBack(x: int)
     modifies this, Repr()
     requires Valid()
     requires forall x | x in Repr() :: allocated(x)
-    
+
     ensures Valid()
     ensures Model() == old(Model()) + [x]
 
@@ -345,18 +341,19 @@ class ArrayListImpl extends ArrayList {
     modifies this, Repr()
     requires Valid()
     requires forall x | x in Repr()::allocated(x)
-    
+
     ensures Valid()
     ensures Model() == old(Model())
-
-    ensures forall x {:trigger x in Repr(), x in old(Repr())} | x in Repr() - old(Repr()) :: fresh(x)
-    ensures fresh(Repr() - old(Repr()))
-    ensures forall x | x in Repr() :: allocated(x)
 
     ensures fresh(it)
     ensures it.Valid()
     ensures it.Parent() == this
     ensures it.Index() == 0
+
+    ensures forall x {:trigger x in Repr(), x in old(Repr())} | x in Repr() - old(Repr()) :: fresh(x)
+    ensures fresh(Repr() - old(Repr()))
+    ensures forall x | x in Repr() :: allocated(x)
+
     ensures Iterators() == {it} + old(Iterators())
     ensures forall it | it in old(iterators) :: old(it.Valid())
       ==> it.Valid() && old(it.Parent()) == it.Parent() && old(it.Index()) == it.Index();
@@ -365,12 +362,13 @@ class ArrayListImpl extends ArrayList {
     iterators := iterators + { it };
   }
 
-  // Deletion of mid, next points to the next element (or past-the-end)
-  method Insert(mid: ListIterator, x: int) returns (newt:ListIterator)
+  // Insertion before mid
+  method Insert(mid: ListIterator, x: int)
     modifies this, Repr()
     requires Valid()
     requires mid.Valid()
     requires mid.Parent() == this
+    requires mid.HasNext()
     requires mid in Iterators()
     requires forall x | x in Repr() :: allocated(x)
 
@@ -381,15 +379,11 @@ class ArrayListImpl extends ArrayList {
     ensures fresh(Repr() - old(Repr()))
     ensures forall x | x in Repr() :: allocated(x)
 
-    ensures fresh(newt)
-    ensures Iterators() == {newt}+old(Iterators())
-    ensures newt.Valid() && newt.Parent()==this && newt.Index()==old(mid.Index())
-    
+    ensures Iterators() == old(Iterators())
     ensures forall it | it in old(iterators) :: old(it.Valid())
       ==> it.Valid() && old(it.Parent()) == it.Parent() && old(it.Index()) == it.Index();
   {
     var midImpl := mid as ArrayListIteratorImpl;
-   
     if (size == elements.Length) {
       Grow(elements.Length * 2);
     }
@@ -398,13 +392,9 @@ class ArrayListImpl extends ArrayList {
     ShiftRight(midImpl.index);
     elements[midImpl.index] := x;
     size := size + 1;
-    assert Model() == Seq.Insert(x, old(Model()), old(mid.Index()));
-
-    newt := midImpl.Copy();
-    iterators := iterators + { newt };
   }
 
-  // Deletion of mid, next points to the next element (or past-the-end)
+  // Deletion of mid
   method Erase(mid: ListIterator) returns (next: ListIterator)
     modifies this, Repr()
     requires Valid()
@@ -413,7 +403,7 @@ class ArrayListImpl extends ArrayList {
     requires mid.HasNext()
     requires mid in Iterators()
     requires forall x | x in Repr() :: allocated(x)
-    
+
     ensures Valid()
     ensures Model() == Seq.Remove(old(Model()), old(mid.Index()))
 
@@ -424,7 +414,7 @@ class ArrayListImpl extends ArrayList {
     ensures fresh(next)
     ensures Iterators() == {next} + old(Iterators())
     ensures forall it | it in old(iterators) :: old(it.Valid()) && old(it.HasNext())
-      ==> it.Valid() && old(it.Parent()) == it.Parent() && old(it.Index()) == it.Index();    
+      ==> it.Valid() && old(it.Parent()) == it.Parent() && old(it.Index()) == it.Index();
     ensures next.Valid() && next.Parent() == this && next.Index() == mid.Index();
   {
     var midImpl := mid as ArrayListIteratorImpl;
@@ -450,20 +440,21 @@ class ArrayListImpl extends ArrayList {
     iterators := iterators + { next };
   }
 
-
   method Grow(newCapacity: nat)
+    modifies this
     requires newCapacity >= elements.Length
     requires Valid()
-    
+    requires forall x | x in Repr() :: allocated(x)
+
     ensures Valid()
     ensures Model() == old(Model())
     ensures this.elements.Length == newCapacity
 
+    ensures Iterators() == old(Iterators())
+
     ensures forall x {:trigger x in Repr(), x in old(Repr())} | x in Repr() - old(Repr()) :: fresh(x)
     ensures fresh(Repr() - old(Repr()))
-    
-    ensures Iterators() == old(Iterators())
-    modifies this
+    ensures forall x | x in Repr() :: allocated(x)
   {
     var newElements := new int[newCapacity];
     var i := 0;
@@ -529,5 +520,4 @@ class ArrayListImpl extends ArrayList {
     }
     assert i == size - 1;
   }
-
 }
